theories/algorithms/KV/KV_Mealy_Binary.v
@@ -1,0 +1,704 @@
+(** Kearns-Vazirani for Mealy machines using binary equality-test discrimination
+    trees.
+    Each internal node tests whether the target observation of a suffix
+    [e] (an [option O.t], via [obs = M.tobs output_lang]) equals a stored value
+    [o]. *)
+
+From lstar Require Import automata.Mealy ListLemmas Teacher RS.
+From Stdlib Require Import List.
+From Stdlib Require Import Lia.
+From Stdlib Require Import PeanoNat.
+From Stdlib Require Import Setoids.Setoid.
+From Stdlib Require Import Eqdep_dec.
+Import ListNotations.
+
+Module KV_Mealy_Binary (s : Symbol) (O : Output) (L : MealyLanguage s O) (Tch : MealyTeacher s O L).
+Import s O L Tch M.
+
+(** Observations derived from the target: [obs q t] is the last output emitted
+    while reading [t] after having consumed [q], or [None] if [t] is empty. *)
+Definition obs : str -> str -> option O.t := M.tobs output_lang.
+Definition mealy_output : str -> s.t -> str -> O.t := M.tgt_last output_lang.
+
+Lemma obs_cons : forall q a w, obs q (a :: w) = Some (mealy_output q a w).
+Proof. reflexivity. Qed.
+
+Lemma obs_nil : forall q, obs q nil = None.
+Proof. reflexivity. Qed.
+
+Lemma obs_single : forall q a, obs q [a] = Some (output_lang q a).
+Proof. reflexivity. Qed.
+
+Lemma tgt_last_prefix : forall tl q c a w,
+    mealy_output q c (tl ++ a :: w) = mealy_output (q ++ (c :: tl)) a w.
+Proof.
+    unfold mealy_output.
+    intros tl. induction tl as [| d tl IH]; intros q c a w; simpl.
+    - reflexivity.
+    - rewrite IH. now rewrite <- app_assoc.
+Qed.
+
+Lemma obs_prefix : forall u a w, obs u (a :: w) = obs nil (u ++ a :: w).
+Proof.
+  intros. unfold obs, tobs.
+  destruct (u ++ a :: w) eqn:E.
+    now apply app_eq_nil in E.
+  f_equal.
+  destruct u as [| c u']; simpl in *; inversion E; subst.
+    reflexivity.
+  change (tgt_last _) with mealy_output. now rewrite tgt_last_prefix.
+Qed.
+
+Lemma obs_shift : forall u a t,
+    t <> nil ->
+    obs u (a :: t) = obs (u ++ [a]) t.
+Proof.
+    intros u a t Ht. destruct t as [| b t']; [contradiction|].
+    unfold obs, M.tobs. reflexivity.
+Qed.
+
+Lemma obs_shift_app : forall t u a,
+    obs u (t ++ [a]) = obs (u ++ t) [a].
+Proof.
+    intros t. induction t as [| c t IH]; intros u a; simpl.
+    - now rewrite app_nil_r.
+    - pose proof (obs_shift u c (t ++ [a])
+                   (fun C => ltac:(now apply app_eq_nil in C))).
+      unfold obs, tobs in *.
+      rewrite H, IH. now rewrite <- app_assoc.
+Qed.
+
+Lemma obs_app_single : forall u t a,
+    obs u (t ++ [a]) = Some (output_lang (u ++ t) a).
+Proof. intros. now rewrite obs_shift_app, obs_single. Qed.
+
+Lemma encodes_obs : forall {state} (m : M.t state),
+    encodes m <-> (forall t, M.mobs m m.(M.initial _) t = obs nil t).
+Proof.
+    intros state m. unfold encodes, obs, M.tobs, M.mobs. split.
+    - intros Henc t. destruct t as [| a w]; [reflexivity|].
+      unfold last_output in Henc. now rewrite Henc.
+    - intros Hobs a w. specialize (Hobs (a :: w)).
+      now inversion Hobs.
+Qed.
+
+Definition obs_eq_dec : forall (x y : option O.t), {x = y} + {x <> y}.
+Proof.
+    intros [x|] [y|].
+    - destruct (O.eq_dec x y); [left; now subst | right; congruence].
+    - right; congruence.
+    - right; congruence.
+    - left; reflexivity.
+Defined.
+
+(** A discrimination tree is a binary tree whose internal nodes hold a
+    discriminator suffix [e] and a target observation [o : option O.t],
+    branching on whether [obs u e] equals [o]; leaves hold an access string. *)
+Inductive dtree : Type :=
+| Leaf (access : str)
+| Node (discrim : str) (o : option O.t) (yes no : dtree).
+
+(** Test performed at an internal node: does [u] observe [o] on [e]? *)
+Definition node_test (u e : str) (o : option O.t) : bool :=
+    if obs_eq_dec (obs u e) o then true else false.
+
+Lemma node_test_true : forall u e o,
+    node_test u e o = true <-> obs u e = o.
+Proof.
+    intros u e o. unfold node_test. destruct (obs_eq_dec (obs u e) o).
+    - split; auto.
+    - split; [discriminate | intro; contradiction].
+Qed.
+
+Lemma node_test_false : forall u e o,
+    node_test u e o = false <-> obs u e <> o.
+Proof.
+    intros u e o. unfold node_test. destruct (obs_eq_dec (obs u e) o).
+    - split; [discriminate | intro C; contradiction].
+    - split; auto.
+Qed.
+
+(** Sifting classifies a string [u] by descending the tree until it reaches
+    the appropriate access node *)
+Fixpoint sift (t : dtree) (u : str) : str :=
+    match t with
+    | Leaf q => q
+    | Node e o yes no =>
+        if node_test u e o then sift yes u else sift no u
+    end.
+
+Fixpoint leaves (t : dtree) : list str :=
+    match t with
+    | Leaf q => [q]
+    | Node _ _ yes no => leaves yes ++ leaves no
+    end.
+
+Fixpoint discriminators (t : dtree) : list str :=
+    match t with
+    | Leaf _ => []
+    | Node e _ yes no => e :: discriminators yes ++ discriminators no
+    end.
+
+(** Sifting always lands on a leaf of the tree *)
+Lemma sift_in_leaves : forall t u, In (sift t u) (leaves t).
+Proof.
+    induction t0 as [q | e o yes IHyes no IHno]; intro u; simpl.
+        now left.
+    destruct (node_test u e o); auto using in_or_app.
+Qed.
+
+(** Tree invariants *)
+
+(** A tree is _consistent_ when every access string sifts to its own leaf *)
+Definition consistent (t : dtree) : Prop :=
+    forall q, In q (leaves t) -> sift t q = q.
+
+(** A tree is _separated_ when any two distinct leaves are told apart by some
+    discriminator of the tree *)
+Definition separated (t : dtree) : Prop :=
+    forall u v,
+        In u (leaves t) -> In v (leaves t) -> u <> v ->
+        exists e, In e (discriminators t)
+               /\ obs u e <> obs v e.
+
+(** A tree is _well-formed_ when each node's discriminator classifies the leaves
+    of its two subtrees: every leaf below the [yes] branch observes [o] on [e],
+    and every leaf below the [no] branch does not. *)
+Fixpoint wf' (t : dtree) : Prop :=
+    match t with
+    | Leaf _ => True
+    | Node e o yes no =>
+        (forall q, In q (leaves yes) -> obs q e = o) /\
+        (forall q, In q (leaves no)  -> obs q e <> o) /\
+        wf' yes /\ wf' no
+    end.
+Definition wf t := wf' t /\ In nil (leaves t).
+
+Definition mem := mem str_eq.
+
+Lemma sift_mem : forall t u, mem (sift t u) (leaves t) = true.
+Proof. intros. apply mem_In, sift_in_leaves. Qed.
+
+Definition make_mealy (t : dtree) : M.t { q | mem q (leaves t) = true }.
+    set (state := { q | mem q (leaves t) = true }).
+    assert (initial : state). {
+        exists (sift t nil). apply sift_mem. }
+    assert (transition : state -> s.t -> state). {
+        intros q a. exists (sift t (proj1_sig q ++ [a])). apply sift_mem. }
+    set (output := fun (q : state) (a : s.t) => output_lang (proj1_sig q) a).
+    assert (mempf : forall x, In x (leaves t) -> mem x (leaves t) = true)
+        by (intros x Hx; now apply mem_In).
+    set (ls := list_with_proof (leaves t) (fun q => mem q (leaves t) = true) mempf).
+    refine {| initial    := initial;
+              transition := transition;
+              output     := output;
+              states     := ls;
+              states_complete := _ |}.
+    intro w.
+    set (qst := fold_left transition w initial).
+    assert (Hin : In (proj1_sig qst) (leaves t))
+        by apply (mem_In str_eq), (proj2_sig qst).
+    assert (Heq : qst = exist _ (proj1_sig qst) (mempf (proj1_sig qst) Hin)). {
+        destruct qst as (q & Hq); simpl.
+        f_equal. apply (UIP_dec Bool.bool_dec). }
+    rewrite Heq.
+    apply (list_with_proof_complete (leaves t) (fun q => mem q (leaves t) = true)).
+    intros. apply UIP_dec, Bool.bool_dec.
+Defined.
+
+Lemma wf_NoDup : forall t, wf t -> NoDup (leaves t).
+Proof.
+    intros. destruct H as (Hwf & _).
+    induction t0 as [q | e o yes IHyes no IHno].
+        simpl. constructor; [intuition | constructor].
+    simpl in Hwf. destruct Hwf as (Hy & Hn & Wy & Wn). simpl.
+    apply NoDup_app_intro; [now apply IHyes | now apply IHno |].
+    intros x Hx Hxn. pose proof (Hy x Hx). pose proof (Hn x Hxn). congruence.
+Qed.
+
+Lemma wf_consistent : forall t, wf t -> consistent t.
+Proof.
+    intros. destruct H as (Hwf & _).
+    induction t0 as [q | e o yes IHyes no IHno]; intros q0 Hin.
+        simpl in Hin. destruct Hin as [H | []]. simpl. assumption.
+    simpl in Hwf. destruct Hwf as (Hy & Hn & Wy & Wn).
+    simpl in Hin. apply in_app_or in Hin. simpl. destruct Hin.
+        rewrite (proj2 (node_test_true q0 e o) (Hy q0 H)). now apply IHyes.
+    rewrite (proj2 (node_test_false q0 e o) (Hn q0 H)). now apply IHno.
+Qed.
+
+Lemma wf_separated : forall t, wf t -> separated t.
+Proof.
+    intros. destruct H as (Hwf & _).
+    induction t0 as [q | e o yes IHyes no IHno]; intros u v Hu Hv Huv.
+        simpl in Hu, Hv. destruct Hu as [-> | []], Hv as [-> | []]. now elim Huv.
+    simpl in Hwf. destruct Hwf as (Hy & Hn & Wy & Wn).
+    simpl in Hu, Hv. apply in_app_or in Hu. apply in_app_or in Hv.
+    destruct Hu as [Hu | Hu], Hv as [Hv | Hv].
+    - destruct (IHyes Wy u v Hu Hv Huv) as (d & Hd & Hdiff).
+      exists d. split; [simpl; right; apply in_or_app; now left | assumption].
+    - exists e. split; [simpl; now left |].
+      rewrite (Hy u Hu). intro C. symmetry in C. now apply (Hn v Hv).
+    - exists e. split; [simpl; now left |].
+      rewrite (Hy v Hv). intro C. now apply (Hn u Hu).
+    - destruct (IHno Wn u v Hu Hv Huv) as (d & Hd & Hdiff).
+      exists d. split; [simpl; right; apply in_or_app; now right | assumption].
+Qed.
+
+(** Set up Shahbaz-Groz counterexample analysis *)
+Module RSS <: MealySG_Setup s O L.
+  Definition obt := { t : dtree | wf t }.
+  Definition P (o : obt) (q : str) : Prop := mem q (leaves (proj1_sig o)) = true.
+  Definition make_mealy (o : obt) : M.t { q | P o q } := make_mealy (proj1_sig o).
+
+  Lemma eps_in_H : forall (o : obt),
+      proj1_sig (make_mealy o).(initial _) = [].
+  Proof.
+    intros (t & Hwf). unfold make_mealy, KV_Mealy_Binary.make_mealy. simpl.
+    apply (wf_consistent t Hwf). now destruct Hwf.
+  Qed.
+
+  Lemma out_correct : forall (o : obt) q a,
+      output _ (make_mealy o) q a = output_lang (proj1_sig q) a.
+  Proof.
+    intros (t & Hwf) q a. unfold make_mealy, KV_Mealy_Binary.make_mealy. reflexivity.
+  Qed.
+
+  Definition obs : str -> str -> option O.t := obs.
+
+  Lemma prediction_is_obs_at_access : forall H w' a,
+      mobs (make_mealy H) (make_mealy H).(initial _) (w' ++ a :: nil)
+        = obs (proj1_sig (run (make_mealy H) w')) (a :: nil).
+  Proof.
+    intros H w' a. rewrite M.mobs_snoc.
+    rewrite out_correct. unfold obs, KV_Mealy_Binary.obs. rewrite obs_single. reflexivity.
+  Qed.
+End RSS.
+
+Module SG := MealySG s O L RSS.
+Import SG.
+
+Fixpoint split_leaf (t : dtree) (target e q_new : str) : dtree :=
+    match t with
+    | Leaf q =>
+        if str_eq q target
+        then Node e (obs q e) (Leaf q) (Leaf q_new)
+        else Leaf q
+    | Node e' o' yes no =>
+        Node e' o' (split_leaf yes target e q_new) (split_leaf no target e q_new)
+    end.
+
+Lemma split_leaves_fwd : forall t target e q_new x,
+    In x (leaves (split_leaf t target e q_new)) ->
+    x = q_new \/ In x (leaves t).
+Proof.
+    induction t0 as [q | e' o' yes IHyes no IHno]; intros target e q_new x H.
+    - simpl in H. destruct (str_eq q target) as [Heq | Hneq]; simpl in H.
+      + destruct H as [-> | [-> | []]]; auto. now right; left.
+      + destruct H as [-> | []]. right; now left.
+    - simpl in H. apply in_app_or in H. destruct H;
+      [destruct (IHyes target e q_new x H) as [Hqn | Hin]|
+       destruct (IHno target e q_new x H) as [Hqn | Hin]]; auto;
+       right; apply in_or_app; auto.
+Qed.
+
+Lemma split_leaf_id : forall t target e q_new,
+    ~ In target (leaves t) ->
+    split_leaf t target e q_new = t.
+Proof.
+    induction t0 as [q | e' o' yes IHyes no IHno]; intros target e q_new Hni; simpl in *.
+    - destruct (str_eq q target); auto.
+      destruct Hni; auto.
+    - f_equal; [apply IHyes | apply IHno]; intro; eauto using in_or_app.
+Qed.
+
+Lemma split_leaves_pres : forall t target e q_new x,
+    In x (leaves t) -> In x (leaves (split_leaf t target e q_new)).
+Proof.
+    induction t0 as [q | e' o' yes IHyes no IHno]; intros target e q_new x H.
+    - simpl in H. destruct H; [|contradiction].
+      simpl. destruct (str_eq q target); subst; [|now left].
+      simpl. now left.
+    - apply in_app_or in H. apply in_or_app.
+      destruct H; auto.
+Qed.
+
+Lemma split_q_new_in : forall t target e q_new,
+    In target (leaves t) -> In q_new (leaves (split_leaf t target e q_new)).
+Proof.
+    induction t0 as [q | e' o' yes IHyes no IHno]; intros target e q_new H.
+    - simpl in H. destruct H; [|contradiction]; subst.
+      simpl. destruct (str_eq target target); [|contradiction].
+      simpl. right; now left.
+    - simpl in H. apply in_app_or in H. simpl. apply in_or_app.
+      destruct H; auto.
+Qed.
+
+(** A well-oriented split preserves distinctness of leaves: [target] occurs once
+    and [q_new] is fresh, so replacing the former by the pair adds no
+    duplicates *)
+Lemma split_NoDup : forall t target e q_new,
+    NoDup (leaves t) -> In target (leaves t) -> ~ In q_new (leaves t) ->
+    NoDup (leaves (split_leaf t target e q_new)).
+Proof.
+    induction t0 as [q | e' o' yes IHyes no IHno]; intros target e q_new HND HinT Hfresh.
+    - simpl in HinT. destruct HinT as [Hq | []]. simpl in Hfresh.
+      assert (Hqn : q_new <> q) by (intro Heq; apply Hfresh; left; congruence).
+      simpl. destruct (str_eq q target) as [_ | Hneq]; [| congruence].
+      simpl. constructor;
+        [ intros [C | []]; congruence
+        | constructor; [intros [] | constructor] ].
+    - simpl in HND, HinT, Hfresh. simpl.
+      pose proof (NoDup_app_l _ _ HND) as NDy.
+      pose proof (NoDup_app_r _ _ HND) as NDn.
+      assert (Hfy : ~ In q_new (leaves yes))
+          by (intro; apply Hfresh, in_or_app; now left).
+      assert (Hfn : ~ In q_new (leaves no))
+          by (intro; apply Hfresh, in_or_app; now right).
+      apply in_app_or in HinT. destruct HinT as [Hin | Hin].
+      + assert (Hnn : ~ In target (leaves no))
+            by now apply (NoDup_app_disj _ _ HND).
+        rewrite (split_leaf_id no target e q_new Hnn).
+        apply NoDup_app_intro; [now apply IHyes | assumption |].
+        intros x Hx Hxn. apply split_leaves_fwd in Hx. destruct Hx as [-> | Hx].
+            now apply Hfn.
+        now apply (NoDup_app_disj _ _ HND x Hx).
+      + assert (Hny : ~ In target (leaves yes))
+            by (intro Hy; apply (NoDup_app_disj _ _ HND target Hy Hin)).
+        rewrite (split_leaf_id yes target e q_new Hny).
+        apply NoDup_app_intro; [assumption | now apply IHno |].
+        intros x Hx Hxn. apply split_leaves_fwd in Hxn. destruct Hxn as [-> | Hxn].
+            now apply Hfy.
+        now apply (NoDup_app_disj _ _ HND x Hx).
+Qed.
+
+Lemma consistent_NoDup_wf' : forall t,
+    NoDup (leaves t) -> consistent t -> wf' t.
+Proof.
+    induction t0 as [q | e o yes IHyes no IHno]; intros HND Hcons; [exact I |].
+    simpl in HND.
+    pose proof (NoDup_app_l _ _ HND) as NDy.
+    pose proof (NoDup_app_r _ _ HND) as NDn.
+    assert (Hdisj : forall x, In x (leaves yes) -> ~ In x (leaves no))
+        by now apply NoDup_app_disj.
+    (* the yes subtree's leaves observe o on e *)
+    assert (Hy : forall q, In q (leaves yes) -> obs q e = o). {
+        intros q Hq. destruct (node_test q e o) eqn:E.
+          now apply node_test_true.
+        exfalso.
+        assert (Hsc : sift (Node e o yes no) q = q)
+            by (apply Hcons; simpl; apply in_or_app; now left).
+        simpl in Hsc. rewrite E in Hsc.
+        apply (Hdisj q Hq). rewrite <- Hsc. apply sift_in_leaves. }
+    (* the no subtree's leaves do not observe o on e *)
+    assert (Hn : forall q, In q (leaves no) -> obs q e <> o). {
+        intros q Hq. destruct (node_test q e o) eqn:E.
+          exfalso.
+          assert (Hsc : sift (Node e o yes no) q = q)
+              by (apply Hcons; simpl; apply in_or_app; now right).
+          simpl in Hsc. rewrite E in Hsc.
+          apply (Hdisj q); [rewrite <- Hsc; apply sift_in_leaves | assumption].
+        now apply node_test_false. }
+    (* and the subtrees are themselves consistent *)
+    assert (Cy : consistent yes). {
+        intros q Hq.
+        assert (Hsc : sift (Node e o yes no) q = q)
+            by (apply Hcons; simpl; apply in_or_app; now left).
+        simpl in Hsc.
+        now rewrite (proj2 (node_test_true q e o) (Hy q Hq)) in Hsc. }
+    assert (Cn : consistent no). {
+        intros q Hq.
+        assert (Hsc : sift (Node e o yes no) q = q)
+            by (apply Hcons; simpl; apply in_or_app; now right).
+        simpl in Hsc.
+        now rewrite (proj2 (node_test_false q e o) (Hn q Hq)) in Hsc. }
+    simpl. repeat split; auto.
+Qed.
+
+(** [split_leaf] preserves the invariant *)
+Lemma split_preserves_wf' : forall t target e q_new,
+    wf' t ->
+    In target (leaves t) ->
+    ~ In q_new (leaves t) ->
+    sift t q_new = target ->
+    obs target e <> obs q_new e ->
+    wf' (split_leaf t target e q_new).
+Proof.
+    induction t0 as [q | e' o' yes IHyes no IHno];
+        intros target e q_new Hwf HinT Hfresh Hsift Hdiff.
+    - simpl in HinT. destruct HinT as [Hq | []]. subst target.
+      simpl. destruct (str_eq q q) as [_ | Hneq]; [| now destruct (Hneq eq_refl)].
+      (* the new node tests obs q e: q lands yes, q_new lands no *)
+      simpl. repeat split.
+      + intros x [Hx | []]. subst x. reflexivity.
+      + intros x [Hx | []]. subst x. intro C. apply Hdiff. now rewrite C.
+    - simpl in Hwf. destruct Hwf as (Hy & Hn & Wy & Wn).
+      simpl in HinT, Hfresh. apply in_app_or in HinT. simpl.
+      assert (Hfy : ~ In q_new (leaves yes))
+          by (intro; apply Hfresh, in_or_app; now left).
+      assert (Hfn : ~ In q_new (leaves no))
+          by (intro; apply Hfresh, in_or_app; now right).
+      destruct HinT as [Hin | Hin].
+      + (* target is in the yes subtree, so the no subtree is untouched *)
+        assert (Hnn : ~ In target (leaves no))
+            by (intro H; pose proof (Hy target Hin); pose proof (Hn target H);
+                congruence).
+        (* q_new sifts toward the yes subtree as well *)
+        assert (Hqe' : node_test q_new e' o' = true). {
+            destruct (node_test q_new e' o') eqn:E; [reflexivity |].
+            destruct Hnn.
+            assert (sift no q_new = target) by (simpl in Hsift; now rewrite E in Hsift).
+            rewrite <- H. apply sift_in_leaves. }
+        assert (Hsy : sift yes q_new = target)
+            by (simpl in Hsift; now rewrite Hqe' in Hsift).
+        rewrite (split_leaf_id no target e q_new Hnn).
+        repeat split; auto.
+        * intros x Hx. apply split_leaves_fwd in Hx. destruct Hx as [-> | Hx].
+            (* x = q_new : its observation on e' equals o', since q_new sifts yes *)
+            now apply node_test_true.
+          now apply Hy.
+      + (* symmetric: target is in the no subtree *)
+        assert (Hny : ~ In target (leaves yes))
+            by (intro H; pose proof (Hy target H); pose proof (Hn target Hin);
+                congruence).
+        assert (Hqe' : node_test q_new e' o' = false). {
+            destruct (node_test q_new e' o') eqn:E; [| reflexivity].
+            destruct Hny.
+            assert (sift yes q_new = target) by (simpl in Hsift; now rewrite E in Hsift).
+            rewrite <- H. apply sift_in_leaves. }
+        assert (Hsn : sift no q_new = target)
+            by (simpl in Hsift; now rewrite Hqe' in Hsift).
+        rewrite (split_leaf_id yes target e q_new Hny).
+        repeat split; auto.
+        * intros x Hx. apply split_leaves_fwd in Hx. destruct Hx as [-> | Hx].
+            (* x = q_new : its observation on e' differs from o', since q_new sifts no *)
+            now apply node_test_false.
+          now apply Hn.
+Qed.
+
+(** Given a tree whose hypothesis mispredicts on a counterexample [w], find a
+    leaf [target] and a fresh non-empty discriminator [e] such that splitting
+    [target] on [e] yields a still well-formed tree. *)
+Theorem find_split :
+    forall (t : dtree) (w : str)
+           (Heps : In nil (leaves t))
+           (Hcons : consistent t)
+           (HND : NoDup (leaves t))
+           (Hce : mobs (make_mealy t) (make_mealy t).(initial _) w <> obs nil w),
+    { target : str &
+    { e : str &
+    { q_new : str |
+        In target (leaves t) /\
+        ~ In q_new (leaves t) /\
+        obs target e <> obs q_new e /\
+        let t' := split_leaf t target e q_new in
+        wf t' }}}.
+Proof.
+    intros t. intros.
+    assert (Hwf : wf t) by (split; [ now apply consistent_NoDup_wf' | easy ]).
+    set (o := exist wf t Hwf : RSS.obt).
+    assert (Hce' : mobs (RSS.make_mealy o) (RSS.make_mealy o).(initial _) w
+                   <> obs nil w) by exact Hce.
+    (* The counterexample is non-empty: peel its last symbol. *)
+    assert (Hne : w <> nil). {
+      intro Hw. subst w. apply Hce. reflexivity. }
+    destruct (exists_last Hne) as (w' & a & Hw). subst w.
+    (* Shahbaz-Groz search: a flip strictly inside w'. *)
+    destruct (sg_partition_binary o w' a Hce')
+        as (k & KCorrect & SKincorrect & Hlt).
+    (* The two adjacent reconstructions differ. *)
+    assert (Dist : sg o w' a k <> sg o w' a (S k)). {
+      unfold correct in KCorrect, SKincorrect.
+      rewrite KCorrect. intro Hbad. apply SKincorrect. now rewrite <- Hbad.
+    }
+    (* Name the k-th symbol of w' and split skipn k w'. *)
+    assert {wk | nth_error w' k = Some wk} as (wk & Hwk). {
+      destruct (nth_error w' k) eqn:E.
+        now exists t0.
+      rewrite nth_error_None in E. lia.
+    }
+    pose proof (skipn_S_wk _ w' k wk Hwk) as Hskipn.
+    set (e := skipn (S k) w' ++ [a]).
+    assert (Htne : e <> nil). {
+      unfold e. intro Hbad.
+      now apply app_eq_nil in Hbad as (_ & Hcontra). }
+    destruct (nth_error_split_sig _ _ _ Hwk) as (l1 & l2 & Hw' & Hlen).
+    assert (Hfirstn : firstn (S k) w' = firstn k w' ++ [wk]). {
+        subst.
+        now rewrite firstn_app, Nat.sub_succ_l, firstn_all2, firstn_cons,
+                    Nat.sub_diag, firstn_0, firstn_len_app by lia.
+    }
+    set (qk1 := pi o w' k ++ [wk]).
+    (* One step of the hypothesis advances from p_k to the leaf [qk1] sifts to *)
+    assert (HSk : pi o w' (S k) = sift t qk1). {
+        unfold pi, qk1, run, RSS.make_mealy, make_mealy. rewrite Hfirstn, fold_left_app.
+        reflexivity.
+    }
+    (* From correctness at k and incorrectness at (S k), the extension and the
+       leaf it sifts to are told apart by the suffix e *)
+    assert (DistQ : obs qk1 e <> obs (sift t qk1) e). {
+      rewrite <- HSk. intro Hbad. apply Dist. unfold sg.
+      rewrite Hskipn. fold e.
+      change ((wk :: skipn (S k) w') ++ [a]) with (wk :: e).
+      unfold RSS.obs. rewrite (obs_shift (pi o w' k) wk e Htne).
+      fold qk1. exact Hbad.
+    }
+    exists (sift t qk1), e, qk1.
+    pose proof (sift_in_leaves t qk1) as HinT.
+    assert (Hfresh : ~ In qk1 (leaves t)). {
+        intro Hin. rewrite (Hcons qk1 Hin) in DistQ. now apply DistQ.
+    }
+    assert (Hdiff : obs (sift t qk1) e <> obs qk1 e) by (intro C; apply DistQ; now rewrite C).
+    assert (Hwf' : wf' t) by (now apply consistent_NoDup_wf').
+    assert (Hwf'' : wf' (split_leaf t (sift t qk1) e qk1))
+        by (now apply split_preserves_wf').
+    repeat split; auto using split_leaves_pres.
+Defined.
+
+(** Each counterexample adds exactly one state *)
+Lemma split_leaf_count : forall t target e q_new,
+    NoDup (leaves t) -> In target (leaves t) -> ~ In q_new (leaves t) ->
+    length (leaves (split_leaf t target e q_new)) = S (length (leaves t)).
+Proof.
+    intros t target e q_new HND HinT Hfresh.
+    assert (ND' : NoDup (leaves (split_leaf t target e q_new)))
+        by now apply split_NoDup.
+    assert (NDc : NoDup (q_new :: leaves t)) by now constructor.
+    assert (I1 : incl (leaves (split_leaf t target e q_new)) (q_new :: leaves t)). {
+        intros x Hx. apply split_leaves_fwd in Hx. destruct Hx as [-> | Hx]; now constructor.
+    }
+    assert (I2 : incl (q_new :: leaves t) (leaves (split_leaf t target e q_new))). {
+        intros x [-> | Hx];
+            [now apply split_q_new_in | now apply split_leaves_pres].
+    }
+    pose proof (NoDup_incl_length ND' I1) as L1.
+    pose proof (NoDup_incl_length NDc I2) as L2.
+    simpl in L1, L2. lia.
+Qed.
+
+Lemma make_mealy_minimal : forall t,
+    wf t ->
+    equiv_query (make_mealy t) = None ->
+    minimal (make_mealy t).
+Proof.
+  intros t Hwf Heq.
+  unfold minimal. split.
+    now apply equiv_query_correct in Heq.
+  intros state' m' H_encodes0.
+  pose proof (proj1 (encodes_obs m') H_encodes0) as H_encodes.
+  assert (H_LHS : List.length (states _ (make_mealy t)) = List.length (leaves t)). {
+    unfold make_mealy. simpl. apply list_with_proof_preserves_len. }
+  rewrite H_LHS.
+  pose proof (wf_separated _ Hwf) as Hsep.
+  pose proof (wf_NoDup _ Hwf) as HND.
+  set (f := fun q => M.run m' q).
+  assert (Hinj : forall u v, In u (leaves t) -> In v (leaves t) ->
+                 u <> v -> f u <> f v). {
+    intros u v Hu Hv Huv Hf.
+    destruct (Hsep u v Hu Hv Huv) as (e & He & Hdiff).
+    apply Hdiff.
+    destruct e as [| a w]; [now rewrite !obs_nil |].
+    rewrite (obs_prefix u a w), (obs_prefix v a w).
+    rewrite <- (H_encodes (u ++ a :: w)), <- (H_encodes (v ++ a :: w)).
+    rewrite (M.mobs_prefix m' u a w), (M.mobs_prefix m' v a w).
+    unfold f in Hf. now rewrite Hf. }
+  rewrite <- (length_map f (leaves t)).
+  apply NoDup_incl_length.
+  - clear - HND Hinj.
+    induction (leaves t) as [| x xs IH]; [constructor|].
+    apply NoDup_cons_iff in HND. destruct HND as [Hnin NDxs]. constructor.
+    + intro HIn. apply in_map_iff in HIn. destruct HIn as (y & Hfy & Hyin).
+      replace x with y in *. contradiction.
+      destruct (str_eq x y) as [e0|n0]; [now symmetry|].
+      exfalso. apply (Hinj x y); [now left | now right | assumption | now symmetry].
+    + apply IH; auto. intros u v Hu Hv. apply Hinj; now right.
+  - intros st Hst. apply in_map_iff in Hst.
+    destruct Hst as (q & <- & _). unfold f. apply M.run_in_states.
+Qed.
+
+Lemma le_min : forall t,
+    wf t ->
+    length (leaves t) <= num_states_in_minimal.
+Proof.
+  intro t. intro Hwf.
+  destruct L.exists_mealy as (state_m & Mm & (Menc0 & Minimal) & Len).
+  rewrite encodes_obs in Menc0. rename Menc0 into Menc.
+  enough (Hle : List.length (leaves t) <= List.length (M.states state_m Mm)) by lia.
+  pose proof (wf_separated _ Hwf) as Hsep.
+  pose proof (wf_NoDup _ Hwf) as HND.
+  set (f := fun q => M.run Mm q).
+  assert (Hinj : forall u v, In u (leaves t) -> In v (leaves t) ->
+                 u <> v -> f u <> f v). {
+    intros u v Hu Hv Huv Hf.
+    destruct (Hsep u v Hu Hv Huv) as (e & He & Hdiff).
+    apply Hdiff.
+    destruct e as [| a w]; [now rewrite !obs_nil |].
+    rewrite (obs_prefix u a w), (obs_prefix v a w).
+    rewrite <- (Menc (u ++ a :: w)), <- (Menc (v ++ a :: w)).
+    rewrite (M.mobs_prefix Mm u a w), (M.mobs_prefix Mm v a w).
+    unfold f in Hf. now rewrite Hf. }
+  rewrite <- (length_map f (leaves t)).
+  apply NoDup_incl_length.
+  - clear - HND Hinj.
+    induction (leaves t) as [| x xs IH]; [constructor|].
+    apply NoDup_cons_iff in HND. destruct HND as [Hnin NDxs]. constructor.
+    + intro HIn. apply in_map_iff in HIn. destruct HIn as (y & Hfy & Hyin).
+      assert (x = y). { destruct (str_eq x y) as [e|n]; [exact e|].
+        exfalso. apply (Hinj x y); [now left | now right | exact n | now symmetry]. }
+      subst y; contradiction.
+    + apply IH; auto. intros u v Hu Hv. apply Hinj; now right.
+  - intros st Hst. apply in_map_iff in Hst.
+    destruct Hst as (q & <- & _). unfold f. apply M.run_in_states.
+Qed.
+
+Lemma full_states_no_ce : forall (t : dtree),
+    wf t ->
+    L.num_states_in_minimal <= List.length (leaves t) ->
+    equiv_query (make_mealy t) = None.
+Proof.
+    intros t Hwf Contra.
+    destruct (equiv_query (make_mealy t)) eqn:Heq; [exfalso | reflexivity].
+    assert (Hce : mobs (make_mealy t) (make_mealy t).(initial _) s <> obs nil s)
+        by (unfold obs; now apply equiv_query_ce).
+    pose proof (wf_consistent _ Hwf) as Hcons.
+    pose proof (wf_NoDup _ Hwf) as HND. destruct Hwf as (Hwf & Heps).
+    destruct (find_split _ s Heps Hcons HND Hce) as
+        (target & e & q_new & In_target & NIn_qnew & Membership & X).
+    cbv zeta in X. destruct X as (Wft' & Heps').
+    pose proof (split_leaf_count t target e q_new HND In_target NIn_qnew) as Hcount.
+    assert (wf (split_leaf t target e q_new)) by now split.
+    pose proof (le_min _ H) as Hcap.
+    rewrite Hcount in Hcap.
+    lia.
+Qed.
+
+(** The main KV implementation. Adds one state per counterexample *)
+Fixpoint kv_learn (fuel : nat) (t : dtree)
+                  (LE : L.num_states_in_minimal - List.length (leaves t) <= fuel)
+                  (Hwf : wf t)
+    : { St : Type & {m : M.t St | minimal m} }.
+    destruct (equiv_query (make_mealy t)) eqn:Heq.
+    - (* counterexample *)
+        destruct fuel as [| n].
+        -- assert (forall x y, x - y <= 0 -> x - y = 0) by lia. apply H in LE. clear H.
+           apply Nat.sub_0_le, full_states_no_ce in LE; auto.
+           rewrite Heq in LE. discriminate.
+        -- assert (Hce : mobs (make_mealy t) (make_mealy t).(initial _) s <> obs nil s)
+                by (unfold obs; now apply equiv_query_ce).
+            pose proof Hwf as Hwf'.
+            destruct Hwf' as (Hwf' & Heps).
+            destruct (find_split t s Heps (wf_consistent t Hwf) (wf_NoDup t Hwf) Hce)
+                as (target & e & q_new & HinT & Hfresh & Hdiff & Hwf'' & Heps').
+            enough (num_states_in_minimal - List.length (leaves (split_leaf t target e q_new)) <= n).
+            eapply (kv_learn n (split_leaf t target e q_new) H (conj Hwf'' Heps')).
+            pose proof (split_leaf_count t target e q_new
+                          (wf_NoDup t Hwf) HinT Hfresh) as Hcount.
+            rewrite Hcount. lia.
+    - eexists. exists (make_mealy t). apply (make_mealy_minimal t Hwf Heq).
+Defined.
+
+(** The learner is seeded with a trivially well-formed tree *)
+Definition mkv (_ : unit) : { St : Type & {m : M.t St | minimal m} } :=
+    kv_learn num_states_in_minimal (Leaf nil) ltac:(lia) (conj I (or_introl eq_refl)).
+
+End KV_Mealy_Binary.
