theories/algorithms/TTT/TTT_Moore_Binary.v
@@ -1,0 +1,722 @@
+(** TTT automata learning for Moore machines, binary equality-test
+    discrimination trees with final/temporary discriminators.
+    https://doi.org/10.1007/978-3-319-11164-3 *)
+
+From Stdlib Require Import Lia PeanoNat Bool.
+From Stdlib Require Import Eqdep_dec.
+From lstar Require Import automata.Moore Teacher ListLemmas RS.
+Import ListNotations.
+
+Module TTT_Moore_Binary (s : Symbol) (O : Output) (L : MooreLanguage s O) (Tch : MooreTeacher s O L).
+Import s L Tch M.
+
+(** Discriminators are tagged with whether they are _final_ or _temporary_ *)
+Inductive disc : Type :=
+| Final (e : str)
+| Temp  (e : str).
+
+Definition disc_str (d : disc) : str :=
+    match d with Final e => e | Temp e => e end.
+
+Inductive ttree : Type :=
+| Leaf (access : str)
+| Node (d : disc) (o : O.t) (yes no : ttree).
+
+(** Test performed at an internal node: does [u] produce output [o] on [e]? *)
+Definition node_test (u e : str) (o : O.t) : bool :=
+    if O.eq_dec (output_lang (u ++ e)) o then true else false.
+
+Lemma node_test_true : forall u e o,
+    node_test u e o = true <-> output_lang (u ++ e) = o.
+Proof.
+    intros u e o. unfold node_test. destruct (O.eq_dec (output_lang (u ++ e)) o).
+    - split; auto.
+    - split; [discriminate | intro; contradiction].
+Qed.
+
+Lemma node_test_false : forall u e o,
+    node_test u e o = false <-> output_lang (u ++ e) <> o.
+Proof.
+    intros u e o. unfold node_test. destruct (O.eq_dec (output_lang (u ++ e)) o).
+    - split; [discriminate | intro C; contradiction].
+    - split; auto.
+Qed.
+
+(** Sifting, as in KV *)
+Fixpoint sift (t : ttree) (u : str) : str :=
+    match t with
+    | Leaf q => q
+    | Node d o yes no =>
+        if node_test u (disc_str d) o then sift yes u else sift no u
+    end.
+
+Fixpoint leaves (t : ttree) : list str :=
+    match t with
+    | Leaf q => [q]
+    | Node _ _ yes no => leaves yes ++ leaves no
+    end.
+
+Fixpoint discriminators (t : ttree) : list disc :=
+    match t with
+    | Leaf _ => []
+    | Node d _ yes no => d :: discriminators yes ++ discriminators no
+    end.
+
+Lemma sift_in_leaves : forall t u, In (sift t u) (leaves t).
+Proof.
+    induction t0 as [q | d o yes IHyes no IHno]; intro u; simpl.
+        now left.
+    destruct (node_test u (disc_str d) o); auto using in_or_app.
+Qed.
+
+(** Tree invariants, as in KV *)
+Definition consistent (t : ttree) : Prop :=
+    forall q, In q (leaves t) -> sift t q = q.
+
+Definition separated (t : ttree) : Prop :=
+    forall u v,
+        In u (leaves t) -> In v (leaves t) -> u <> v ->
+        exists d, In d (discriminators t)
+                /\ output_lang (u ++ disc_str d) <> output_lang (v ++ disc_str d).
+
+Fixpoint wf' (t : ttree) : Prop :=
+    match t with
+    | Leaf _ => True
+    | Node d o yes no =>
+        (forall q, In q (leaves yes) -> output_lang (q ++ disc_str d) = o) /\
+        (forall q, In q (leaves no)  -> output_lang (q ++ disc_str d) <> o) /\
+        wf' yes /\ wf' no
+    end.
+Definition wf t := wf' t /\ In nil (leaves t).
+
+(** A discrimination tree is _finalized_ if all of its internal nodes are
+    final *)
+Fixpoint finalized (t : ttree) : Prop :=
+    match t with
+    | Leaf _ => True
+    | Node (Final _) _ yes no => finalized yes /\ finalized no
+    | _ => False
+    end.
+
+Definition mem := mem str_eq.
+
+Lemma sift_mem : forall t u, mem (sift t u) (leaves t) = true.
+Proof. intros. apply mem_In, sift_in_leaves. Qed.
+
+Definition make_moore (t : ttree) : M.t { q | mem q (leaves t) = true }.
+    set (state := { q | mem q (leaves t) = true }).
+    assert (initial : state). {
+        exists (sift t nil). apply sift_mem. }
+    assert (transition : state -> s.t -> state). {
+        intros q a. exists (sift t (proj1_sig q ++ [a])). apply sift_mem. }
+    set (output := fun (q : state) => output_lang (proj1_sig q)).
+    assert (mempf : forall x, In x (leaves t) -> mem x (leaves t) = true)
+        by (intros x Hx; now apply mem_In).
+    set (ls := list_with_proof (leaves t) (fun q => mem q (leaves t) = true) mempf).
+    refine {| initial    := initial;
+              transition := transition;
+              output     := output;
+              states     := ls;
+              states_complete := _ |}.
+    intro w.
+    set (qst := fold_left transition w initial).
+    assert (Hin : In (proj1_sig qst) (leaves t))
+        by apply (mem_In str_eq), (proj2_sig qst).
+    assert (Heq : qst = exist _ (proj1_sig qst) (mempf (proj1_sig qst) Hin)). {
+        destruct qst as (q & Hq); simpl.
+        f_equal. apply (UIP_dec Bool.bool_dec). }
+    rewrite Heq.
+    apply (list_with_proof_complete (leaves t) (fun q => mem q (leaves t) = true)).
+    intros. apply UIP_dec, Bool.bool_dec.
+Defined.
+
+Lemma wf_NoDup : forall t, wf t -> NoDup (leaves t).
+Proof.
+    intros. destruct H as (Hwf & _).
+    induction t0 as [q | d o yes IHyes no IHno].
+        simpl. constructor; [intuition | constructor].
+    simpl in Hwf. destruct Hwf as (Hy & Hn & Wy & Wn). simpl.
+    apply NoDup_app_intro; [now apply IHyes | now apply IHno |].
+    intros x Hx Hxn. pose proof (Hy x Hx). pose proof (Hn x Hxn). congruence.
+Qed.
+
+Lemma wf_consistent : forall t, wf t -> consistent t.
+Proof.
+    intros. destruct H as (Hwf & _).
+    induction t0 as [q | d o yes IHyes no IHno]; intros q0 Hin.
+        simpl in Hin. destruct Hin as [H | []]. simpl. assumption.
+    simpl in Hwf. destruct Hwf as (Hy & Hn & Wy & Wn).
+    simpl in Hin. apply in_app_or in Hin. simpl. destruct Hin.
+        rewrite (proj2 (node_test_true q0 (disc_str d) o) (Hy q0 H)). now apply IHyes.
+    rewrite (proj2 (node_test_false q0 (disc_str d) o) (Hn q0 H)). now apply IHno.
+Qed.
+
+Lemma wf_separated : forall t, wf t -> separated t.
+Proof.
+    intros. destruct H as (Hwf & _).
+    induction t0 as [q | d o yes IHyes no IHno]; intros u v Hu Hv Huv.
+        simpl in Hu, Hv. destruct Hu as [-> | []], Hv as [-> | []]. now elim Huv.
+    simpl in Hwf. destruct Hwf as (Hy & Hn & Wy & Wn).
+    simpl in Hu, Hv. apply in_app_or in Hu. apply in_app_or in Hv.
+    destruct Hu as [Hu | Hu], Hv as [Hv | Hv].
+    - destruct (IHyes Wy u v Hu Hv Huv) as (d' & Hd & Hdiff).
+      exists d'. split; [simpl; right; apply in_or_app; now left | assumption].
+    - exists d. split; [simpl; now left |].
+      rewrite (Hy u Hu). intro C. symmetry in C. now apply (Hn v Hv).
+    - exists d. split; [simpl; now left |].
+      rewrite (Hy v Hv). intro C. now apply (Hn u Hu).
+    - destruct (IHno Wn u v Hu Hv Huv) as (d' & Hd & Hdiff).
+      exists d'. split; [simpl; right; apply in_or_app; now right | assumption].
+Qed.
+
+(** Set up Rivest-Schapire counterexample analysis *)
+Module RSS <: MooreRS_Setup s O L.
+  Definition obt := { o : ttree | wf o }.
+  Definition P (o : obt) (q : str) : Prop := mem q (leaves (proj1_sig o)) = true.
+  Definition make_moore (o : obt) : M.t { q | P o q } := make_moore (proj1_sig o).
+
+  Lemma eps_in_H : forall (o : obt),
+      proj1_sig (make_moore o).(initial _) = [].
+  Proof.
+    intros (t & Hwf). unfold make_moore, TTT_Moore_Binary.make_moore. simpl.
+    apply (wf_consistent t Hwf). now destruct Hwf.
+  Qed.
+
+  Lemma out_correct : forall (o : obt) q,
+      output _ (make_moore o) q = output_lang (proj1_sig q).
+  Proof.
+    intros (t & Hwf) q. unfold make_moore, TTT_Moore_Binary.make_moore. reflexivity.
+  Qed.
+End RSS.
+
+Module RSan := MooreRS s O L RSS.
+Import RSan.
+
+Fixpoint split_leaf (t : ttree) (target e q_new : str) : ttree :=
+    match t with
+    | Leaf q =>
+        if str_eq q target
+        then Node (Temp e) (output_lang (q ++ e)) (Leaf q) (Leaf q_new)
+        else Leaf q
+    | Node d o yes no =>
+        Node d o (split_leaf yes target e q_new) (split_leaf no target e q_new)
+    end.
+
+Lemma split_leaves_fwd : forall t target e q_new x,
+    In x (leaves (split_leaf t target e q_new)) ->
+    x = q_new \/ In x (leaves t).
+Proof.
+    induction t0 as [q | d o yes IHyes no IHno]; intros target e q_new x H.
+    - simpl in H. destruct (str_eq q target) as [Heq | Hneq]; simpl in H.
+      + destruct H as [-> | [-> | []]]; auto. now right; left.
+      + destruct H as [-> | []]. right; now left.
+    - simpl in H. apply in_app_or in H. destruct H;
+      [destruct (IHyes target e q_new x H) as [Hqn | Hin]|
+       destruct (IHno target e q_new x H) as [Hqn | Hin]]; auto;
+       right; apply in_or_app; auto.
+Qed.
+
+Lemma split_leaf_id : forall t target e q_new,
+    ~ In target (leaves t) ->
+    split_leaf t target e q_new = t.
+Proof.
+    induction t0 as [q | d o yes IHyes no IHno]; intros target e q_new Hni; simpl in *.
+    - destruct (str_eq q target); auto.
+      destruct Hni; auto.
+    - f_equal; [apply IHyes | apply IHno]; intro; eauto using in_or_app.
+Qed.
+
+Lemma split_leaves_pres : forall t target e q_new x,
+    In x (leaves t) -> In x (leaves (split_leaf t target e q_new)).
+Proof.
+    induction t0 as [q | d o yes IHyes no IHno]; intros target e q_new x H.
+    - simpl in H. destruct H; [|contradiction].
+      simpl. destruct (str_eq q target); subst; [|now left].
+      simpl. now left.
+    - apply in_app_or in H. apply in_or_app.
+      destruct H; auto.
+Qed.
+
+Lemma split_q_new_in : forall t target e q_new,
+    In target (leaves t) -> In q_new (leaves (split_leaf t target e q_new)).
+Proof.
+    induction t0 as [q | d o yes IHyes no IHno]; intros target e q_new H.
+    - simpl in H. destruct H; [|contradiction]; subst.
+      simpl. destruct (str_eq target target); [|contradiction].
+      simpl. right; now left.
+    - simpl in H. apply in_app_or in H. simpl. apply in_or_app.
+      destruct H; auto.
+Qed.
+
+Lemma split_NoDup : forall t target e q_new,
+    NoDup (leaves t) -> In target (leaves t) -> ~ In q_new (leaves t) ->
+    NoDup (leaves (split_leaf t target e q_new)).
+Proof.
+    induction t0 as [q | d o yes IHyes no IHno]; intros target e q_new HND HinT Hfresh.
+    - simpl in HinT. destruct HinT as [Hq | []]. simpl in Hfresh.
+      assert (Hqn : q_new <> q) by (intro Heq; apply Hfresh; left; congruence).
+      simpl. destruct (str_eq q target) as [_ | Hneq]; [| congruence].
+      simpl. constructor;
+        [ intros [C | []]; congruence
+        | constructor; [intros [] | constructor] ].
+    - simpl in HND, HinT, Hfresh. simpl.
+      pose proof (NoDup_app_l _ _ HND) as NDy.
+      pose proof (NoDup_app_r _ _ HND) as NDn.
+      assert (Hfy : ~ In q_new (leaves yes))
+          by (intro; apply Hfresh, in_or_app; now left).
+      assert (Hfn : ~ In q_new (leaves no))
+          by (intro; apply Hfresh, in_or_app; now right).
+      apply in_app_or in HinT. destruct HinT as [Hin | Hin].
+      + assert (Hnn : ~ In target (leaves no))
+            by now apply (NoDup_app_disj _ _ HND).
+        rewrite (split_leaf_id no target e q_new Hnn).
+        apply NoDup_app_intro; [now apply IHyes | assumption |].
+        intros x Hx Hxn. apply split_leaves_fwd in Hx. destruct Hx as [-> | Hx].
+            now apply Hfn.
+        now apply (NoDup_app_disj _ _ HND x Hx).
+      + assert (Hny : ~ In target (leaves yes))
+            by (intro Hy; apply (NoDup_app_disj _ _ HND target Hy Hin)).
+        rewrite (split_leaf_id yes target e q_new Hny).
+        apply NoDup_app_intro; [assumption | now apply IHno |].
+        intros x Hx Hxn. apply split_leaves_fwd in Hxn. destruct Hxn as [-> | Hxn].
+            now apply Hfy.
+        now apply (NoDup_app_disj _ _ HND x Hx).
+Qed.
+
+Lemma consistent_NoDup_wf' : forall t,
+    NoDup (leaves t) -> consistent t -> wf' t.
+Proof.
+    induction t0 as [q | d o yes IHyes no IHno]; intros HND Hcons; [exact I |].
+    simpl in HND.
+    pose proof (NoDup_app_l _ _ HND) as NDy.
+    pose proof (NoDup_app_r _ _ HND) as NDn.
+    assert (Hdisj : forall x, In x (leaves yes) -> ~ In x (leaves no))
+        by now apply NoDup_app_disj.
+    assert (Hy : forall q, In q (leaves yes) -> output_lang (q ++ disc_str d) = o). {
+        intros q Hq. destruct (node_test q (disc_str d) o) eqn:E.
+          now apply node_test_true.
+        exfalso.
+        assert (Hsc : sift (Node d o yes no) q = q)
+            by (apply Hcons; simpl; apply in_or_app; now left).
+        simpl in Hsc. rewrite E in Hsc.
+        apply (Hdisj q Hq). rewrite <- Hsc. apply sift_in_leaves. }
+    assert (Hn : forall q, In q (leaves no) -> output_lang (q ++ disc_str d) <> o). {
+        intros q Hq. destruct (node_test q (disc_str d) o) eqn:E.
+          exfalso.
+          assert (Hsc : sift (Node d o yes no) q = q)
+              by (apply Hcons; simpl; apply in_or_app; now right).
+          simpl in Hsc. rewrite E in Hsc.
+          apply (Hdisj q); [rewrite <- Hsc; apply sift_in_leaves | assumption].
+        now apply node_test_false. }
+    assert (Cy : consistent yes). {
+        intros q Hq.
+        assert (Hsc : sift (Node d o yes no) q = q)
+            by (apply Hcons; simpl; apply in_or_app; now left).
+        simpl in Hsc.
+        now rewrite (proj2 (node_test_true q (disc_str d) o) (Hy q Hq)) in Hsc. }
+    assert (Cn : consistent no). {
+        intros q Hq.
+        assert (Hsc : sift (Node d o yes no) q = q)
+            by (apply Hcons; simpl; apply in_or_app; now right).
+        simpl in Hsc.
+        now rewrite (proj2 (node_test_false q (disc_str d) o) (Hn q Hq)) in Hsc. }
+    simpl. repeat split; auto.
+Qed.
+
+Lemma split_preserves_wf' : forall t target e q_new,
+    wf' t ->
+    In target (leaves t) ->
+    ~ In q_new (leaves t) ->
+    sift t q_new = target ->
+    output_lang (target ++ e) <> output_lang (q_new ++ e) ->
+    wf' (split_leaf t target e q_new).
+Proof.
+    induction t0 as [q | d o yes IHyes no IHno];
+        intros target e q_new Hwf HinT Hfresh Hsift Hdiff.
+    - simpl in HinT. destruct HinT as [Hq | []]. subst target.
+      simpl. destruct (str_eq q q) as [_ | Hneq]; [| now destruct (Hneq eq_refl)].
+      simpl. repeat split.
+      + intros x [Hx | []]. subst x. reflexivity.
+      + intros x [Hx | []]. subst x. intro C. apply Hdiff. now rewrite C.
+    - simpl in Hwf. destruct Hwf as (Hy & Hn & Wy & Wn).
+      simpl in HinT, Hfresh. apply in_app_or in HinT. simpl.
+      assert (Hfy : ~ In q_new (leaves yes))
+          by (intro; apply Hfresh, in_or_app; now left).
+      assert (Hfn : ~ In q_new (leaves no))
+          by (intro; apply Hfresh, in_or_app; now right).
+      destruct HinT as [Hin | Hin].
+      + assert (Hnn : ~ In target (leaves no))
+            by (intro H; pose proof (Hy target Hin); pose proof (Hn target H);
+                congruence).
+        assert (Hqe' : node_test q_new (disc_str d) o = true). {
+            destruct (node_test q_new (disc_str d) o) eqn:E; [reflexivity |].
+            destruct Hnn.
+            assert (sift no q_new = target) by (simpl in Hsift; now rewrite E in Hsift).
+            rewrite <- H. apply sift_in_leaves. }
+        assert (Hsy : sift yes q_new = target)
+            by (simpl in Hsift; now rewrite Hqe' in Hsift).
+        rewrite (split_leaf_id no target e q_new Hnn).
+        repeat split; auto.
+        * intros x Hx. apply split_leaves_fwd in Hx. destruct Hx as [-> | Hx].
+            now apply node_test_true.
+          now apply Hy.
+      + assert (Hny : ~ In target (leaves yes))
+            by (intro H; pose proof (Hy target H); pose proof (Hn target Hin);
+                congruence).
+        assert (Hqe' : node_test q_new (disc_str d) o = false). {
+            destruct (node_test q_new (disc_str d) o) eqn:E; [| reflexivity].
+            destruct Hny.
+            assert (sift yes q_new = target) by (simpl in Hsift; now rewrite E in Hsift).
+            rewrite <- H. apply sift_in_leaves. }
+        assert (Hsn : sift no q_new = target)
+            by (simpl in Hsift; now rewrite Hqe' in Hsift).
+        rewrite (split_leaf_id yes target e q_new Hny).
+        repeat split; auto.
+        * intros x Hx. apply split_leaves_fwd in Hx. destruct Hx as [-> | Hx].
+            now apply node_test_false.
+          now apply Hn.
+Qed.
+
+Theorem find_split :
+    forall (t : ttree) (w : str)
+           (Heps : In nil (leaves t))
+           (Hcons : consistent t)
+           (HND : NoDup (leaves t))
+           (Hce : output_string (make_moore t) w <> output_lang w),
+    { target : str &
+    { e : str &
+    { q_new : str |
+        In target (leaves t) /\
+        ~ In q_new (leaves t) /\
+        output_lang (target ++ e) <> output_lang (q_new ++ e) /\
+        let t' := split_leaf t target e q_new in
+        wf t' }}}.
+Proof.
+    intros t. intros.
+    assert (Hwf : wf t) by (split; [ now apply consistent_NoDup_wf' | easy ]).
+    destruct (partition_binary (exist _ t Hwf) w Hce)
+      as (k & Kcorrect & SKincorrect).
+    assert (Hlt : k < length w). {
+        destruct (Nat.le_gt_cases (length w) k) as [Hle |]; [| assumption].
+        destruct SKincorrect. unfold correct, pi in *.
+        rewrite firstn_all2, skipn_all2, app_nil_r by lia.
+        now rewrite firstn_all2, skipn_all2, app_nil_r in Kcorrect by lia.
+    }
+    assert {wk | nth_error w k = Some wk}. {
+        destruct (nth_error w k) eqn:E.
+            now exists t0.
+        rewrite nth_error_None in E. lia.
+    } destruct X as (wk & Hwk).
+    destruct (nth_error_split_sig _ _ _ Hwk) as (l1 & l2 & Hw & Hlen).
+    assert (Hfirstn : firstn (S k) w = firstn k w ++ [wk]). {
+        subst.
+        now rewrite firstn_app, Nat.sub_succ_l, firstn_all2, firstn_cons,
+                    Nat.sub_diag, firstn_0, firstn_len_app by lia.
+    }
+    set (o := exist wf t Hwf : RSS.obt).
+    set (qk1 := pi o w k ++ [wk]).
+    exists (sift t qk1), (skipn (S k) w), qk1.
+    assert (HSk : pi o w (S k) = sift t qk1). {
+        unfold pi, qk1, run, make_moore. rewrite Hfirstn, fold_left_app.
+        reflexivity.
+    }
+    assert (Hgk : output_lang (qk1 ++ skipn (S k) w) = output_lang w). {
+        unfold correct in Kcorrect.
+        rewrite (skipn_S_wk _ _ _ _ Hwk) in Kcorrect.
+        unfold qk1. now rewrite <- app_assoc.
+    }
+    assert (Hgk1 : output_lang (sift t qk1 ++ skipn (S k) w) <> output_lang w). {
+        rewrite <- HSk. now unfold correct in SKincorrect.
+    }
+    pose proof (sift_in_leaves t qk1) as HinT.
+    assert (Hfresh : ~ In qk1 (leaves t)). {
+        intro Hin. apply Hgk1. now rewrite (Hcons qk1 Hin).
+    }
+    assert (Hdiff : output_lang (sift t qk1 ++ skipn (S k) w)
+                  <> output_lang (qk1 ++ skipn (S k) w)) by now rewrite Hgk.
+    assert (Hwf' : wf' t) by (now apply consistent_NoDup_wf').
+    assert (Hwf'' : wf' (split_leaf t (sift t qk1) (skipn (S k) w) qk1))
+        by (now apply split_preserves_wf').
+    repeat split; auto using split_leaves_pres.
+Defined.
+
+Lemma split_leaf_count : forall t target e q_new,
+    NoDup (leaves t) -> In target (leaves t) -> ~ In q_new (leaves t) ->
+    List.length (leaves (split_leaf t target e q_new)) = S (List.length (leaves t)).
+Proof.
+    intros t target e q_new HND HinT Hfresh.
+    assert (ND' : NoDup (leaves (split_leaf t target e q_new)))
+        by now apply split_NoDup.
+    assert (NDc : NoDup (q_new :: leaves t)) by now constructor.
+    assert (I1 : incl (leaves (split_leaf t target e q_new)) (q_new :: leaves t)). {
+        intros x Hx. apply split_leaves_fwd in Hx. destruct Hx as [-> | Hx]; now constructor.
+    }
+    assert (I2 : incl (q_new :: leaves t) (leaves (split_leaf t target e q_new))). {
+        intros x [-> | Hx];
+            [now apply split_q_new_in | now apply split_leaves_pres].
+    }
+    pose proof (NoDup_incl_length ND' I1) as Ln1.
+    pose proof (NoDup_incl_length NDc I2) as Ln2.
+    simpl in Ln1, Ln2. lia.
+Qed.
+
+Lemma make_moore_minimal : forall t,
+    wf t ->
+    equiv_query (make_moore t) = None ->
+    minimal (make_moore t).
+Proof.
+  intros t Hwf Heq.
+  unfold minimal. split.
+    now apply equiv_query_correct in Heq.
+  intros state' m' H_encodes.
+  assert (H_LHS : List.length (states _ (make_moore t)) = List.length (leaves t)). {
+    unfold make_moore. simpl. apply list_with_proof_preserves_len. }
+  rewrite H_LHS.
+  pose proof (wf_separated _ Hwf) as Hsep.
+  pose proof (wf_consistent _ Hwf) as Hcons.
+  pose proof (wf_NoDup _ Hwf) as HND.
+  set (f := fun q => M.run m' q).
+  assert (Hinj : forall u v, In u (leaves t) -> In v (leaves t) ->
+                 u <> v -> f u <> f v). {
+    intros u v Hu Hv Huv Hf.
+    destruct (Hsep u v Hu Hv Huv) as (d & Hd & Hdiff).
+    apply Hdiff.
+    assert (Hsplit : forall x,
+              M.output_string m' (x ++ disc_str d)
+              = m'.(M.output _) (fold_left m'.(M.transition _) (disc_str d) (f x)))
+      by (intro x; unfold M.output_string, M.run, f; now rewrite fold_left_app).
+    assert (Hout : M.output_string m' (u ++ disc_str d)
+                 = M.output_string m' (v ++ disc_str d))
+      by (rewrite !Hsplit; unfold f in *; now rewrite Hf).
+    rewrite <- (H_encodes (u ++ disc_str d)), <- (H_encodes (v ++ disc_str d)). assumption. }
+  rewrite <- (length_map f (leaves t)).
+  apply NoDup_incl_length.
+  - clear - HND Hinj.
+    induction (leaves t) as [| x xs IH]; [constructor|].
+    apply NoDup_cons_iff in HND. destruct HND as [Hnin NDxs]. constructor.
+    + intro HIn. apply in_map_iff in HIn. destruct HIn as (y & Hfy & Hyin).
+      replace x with y in *. contradiction.
+      destruct (str_eq x y) as [e0|n0]; [now symmetry|].
+      exfalso. apply (Hinj x y); [now left | now right | assumption | now symmetry].
+    + apply IH; auto. intros u v Hu Hv. apply Hinj; now right.
+  - intros st Hst. apply in_map_iff in Hst.
+    destruct Hst as (q & <- & _). unfold f. apply M.run_in_states.
+Qed.
+
+Lemma le_min : forall t,
+    wf t ->
+    List.length (leaves t) <= num_states_in_minimal.
+Proof.
+  intro t. intro Hwf.
+  destruct L.exists_moore as (state_m & Mm & [Menc Minimal] & Len).
+  enough (Hle : List.length (leaves t) <= List.length (M.states state_m Mm)) by lia.
+  pose proof (wf_separated _ Hwf) as Hsep.
+  pose proof (wf_NoDup _ Hwf) as HND.
+  set (f := fun q => M.run Mm q).
+  assert (Hinj : forall u v, In u (leaves t) -> In v (leaves t) ->
+                 u <> v -> f u <> f v). {
+    intros u v Hu Hv Huv Hf.
+    destruct (Hsep u v Hu Hv Huv) as (d & Hd & Hdiff).
+    apply Hdiff.
+    assert (Hsplit : forall x,
+              M.output_string Mm (x ++ disc_str d)
+              = Mm.(M.output _) (fold_left Mm.(M.transition _) (disc_str d) (f x)))
+      by (intro x; unfold M.output_string, M.run, f; now rewrite fold_left_app).
+    assert (Hout : M.output_string Mm (u ++ disc_str d)
+                 = M.output_string Mm (v ++ disc_str d))
+      by (rewrite !Hsplit; unfold f in *; now rewrite Hf).
+    rewrite <- (Menc (u ++ disc_str d)), <- (Menc (v ++ disc_str d)). assumption. }
+  rewrite <- (length_map f (leaves t)).
+  apply NoDup_incl_length.
+  - clear - HND Hinj.
+    induction (leaves t) as [| x xs IH]; [constructor|].
+    apply NoDup_cons_iff in HND. destruct HND as [Hnin NDxs]. constructor.
+    + intro HIn. apply in_map_iff in HIn. destruct HIn as (y & Hfy & Hyin).
+      assert (x = y). { destruct (str_eq x y) as [e|n]. assumption.
+        exfalso. apply (Hinj x y); [now left | now right | assumption | now symmetry]. }
+      subst y; contradiction.
+    + apply IH; auto. intros u v Hu Hv. apply Hinj; now right.
+  - intros st Hst. apply in_map_iff in Hst.
+    destruct Hst as (q & <- & _). unfold f. apply M.run_in_states.
+Qed.
+
+Lemma full_states_no_ce : forall (t : ttree),
+    wf t ->
+    L.num_states_in_minimal <= List.length (leaves t) ->
+    equiv_query (make_moore t) = None.
+Proof.
+    intros t Hwf Contra.
+    destruct (equiv_query (make_moore t)) eqn:Heq; [exfalso | reflexivity].
+    assert (Hce : output_string (make_moore t) s <> output_lang s)
+        by now apply equiv_query_ce.
+    pose proof (wf_separated _ Hwf) as Hsep.
+    pose proof (wf_consistent _ Hwf) as Hcons.
+    pose proof (wf_NoDup _ Hwf) as HND. destruct Hwf as (Hwf & Heps).
+    destruct (find_split _ s Heps Hcons HND Hce) as
+        (target & e & q_new & In_target & NIn_qnew & Membership & X).
+    cbv zeta in X. destruct X as (Wft' & Heps').
+    pose proof (split_leaf_count t target e q_new HND In_target NIn_qnew) as Hcount.
+    assert (wf (split_leaf t target e q_new)) by now split.
+    pose proof (le_min _ H) as Hcap.
+    rewrite Hcount in Hcap.
+    lia.
+Qed.
+
+Section Finalize.
+  Definition bisects e o l r : bool :=
+    (forallb (fun q => if O.eq_dec (output_lang (q ++ e)) o then true else false) (leaves l)) &&
+    (forallb (fun q => if O.eq_dec (output_lang (q ++ e)) o then false else true) (leaves r)).
+
+  Fixpoint suffixes (e : str) : list str :=
+    e :: match e with
+         | [] => []
+         | _ :: e' => suffixes e'
+         end.
+
+  (** Among the suffixes of [e], pick the shortest that still bisects [l]/[r]
+      with the same output [o]. If none does, fall back to [e]. *)
+  Definition choose (e : str) (o : O.t) (l r : ttree) : str :=
+    match find (fun e' => bisects e' o l r) (rev (suffixes e)) with
+    | Some e' => e'
+    | None    => e
+    end.
+
+  Fixpoint finalize (t : ttree) : ttree :=
+    match t with
+    | Leaf q => Leaf q
+    | Node (Final e) o yes no => Node (Final e) o (finalize yes) (finalize no)
+    | Node (Temp e) o yes no =>
+        let yes' := finalize yes in
+        let no'  := finalize no in
+        Node (Final (choose e o yes' no')) o yes' no'
+    end.
+
+  Lemma finalize_leaves : forall t, leaves (finalize t) = leaves t.
+  Proof.
+    induction t0 as [q | d o yes IHyes no IHno]; simpl.
+        reflexivity.
+    destruct d; simpl; now rewrite IHyes, IHno.
+  Qed.
+
+  Lemma wf_bisects_impl_bisects :
+    forall e o yes no,
+        (forall q : str, In q (leaves yes) -> output_lang (q ++ e) = o) ->
+        (forall q : str, In q (leaves no)  -> output_lang (q ++ e) <> o) ->
+        bisects e o yes no = true.
+  Proof.
+    intros e o yes no Hy Hn.
+    unfold bisects. apply andb_true_iff. split; apply forallb_forall; intros q Hq.
+    - specialize (Hy q Hq). destruct (O.eq_dec (output_lang (q ++ e)) o); congruence.
+    - specialize (Hn q Hq). destruct (O.eq_dec (output_lang (q ++ e)) o); congruence.
+  Qed.
+
+  Lemma bisects_impl_clauses :
+    forall e o yes no,
+      bisects e o yes no = true ->
+      (forall q, In q (leaves yes) -> output_lang (q ++ e) = o) /\
+      (forall q, In q (leaves no)  -> output_lang (q ++ e) <> o).
+  Proof.
+    unfold bisects. intros e o yes no H. apply andb_true_iff in H as [HL HR].
+    rewrite forallb_forall in HL, HR. split.
+    - intros q Hq. specialize (HL q Hq).
+      destruct (O.eq_dec (output_lang (q ++ e)) o); [assumption | discriminate].
+    - intros q Hq. specialize (HR q Hq).
+      destruct (O.eq_dec (output_lang (q ++ e)) o); [discriminate | assumption].
+  Qed.
+
+  Lemma suffixes_length : forall e e',
+    In e' (suffixes e) -> List.length e' <= List.length e.
+  Proof.
+    induction e as [| a e IH]; intros e' Hin; simpl in Hin.
+    - destruct Hin as [<- | []]. reflexivity.
+    - destruct Hin as [<- | Hin].
+      + reflexivity.
+      + simpl. apply le_S. now apply IH.
+  Qed.
+
+  Lemma choose_correct : forall e o l r,
+    bisects e o l r = true ->
+    bisects (choose e o l r) o l r = true /\
+    List.length (choose e o l r) <= List.length e.
+  Proof.
+    intros e o l r He. unfold choose.
+    destruct (find (fun e' => bisects e' o l r) (rev (suffixes e))) eqn:F.
+    - apply find_some in F as [Hin Hbis].
+      apply in_rev in Hin. auto using suffixes_length.
+    - now split.
+  Qed.
+
+  Lemma finalize_preserves_wf :
+    forall t, wf t -> wf (finalize t).
+  Proof.
+    intros t H. destruct H as [H Heps]. unfold wf. split;
+        [clear Heps | now rewrite finalize_leaves].
+    induction t as [q | d o yes IHyes no IHno]; simpl in *.
+        exact I.
+    destruct H as (DL & DR & Hwfy & Hwfn).
+    rewrite <- (finalize_leaves yes) in DL.
+    rewrite <- (finalize_leaves no) in DR.
+    destruct d; simpl.
+    - repeat split; auto.
+    - assert (Hbis : bisects e o (finalize yes) (finalize no) = true)
+          by now apply wf_bisects_impl_bisects.
+      destruct (choose_correct e o (finalize yes) (finalize no) Hbis) as [Hchb _].
+      apply bisects_impl_clauses in Hchb as [HL HR].
+      repeat split; auto.
+  Qed.
+
+  Lemma choose_length : forall e o l r,
+    List.length (choose e o l r) <= List.length e.
+  Proof.
+    intros e o l r. unfold choose.
+    destruct (find (fun e' => bisects e' o l r) (rev (suffixes e))) eqn:F;
+        [|reflexivity].
+    apply find_some in F as [Hin _]. apply in_rev in Hin.
+    now apply suffixes_length.
+  Qed.
+End Finalize.
+
+Section Learner.
+  Definition ttt_step (t : ttree) (target e q_new : str) : ttree :=
+    finalize (split_leaf t target e q_new).
+
+  Fixpoint ttt_learn (fuel : nat) (t : ttree)
+                   (LE : L.num_states_in_minimal - List.length (leaves t) <= fuel)
+                   (Hwf : wf t)
+  : { St : Type & {m : M.t St | minimal m} }.
+  Proof.
+    destruct (equiv_query (make_moore t)) eqn:Heq.
+    - destruct fuel as [| n].
+        + assert (forall x y, x - y <= 0 -> x - y = 0) by lia.
+          apply H in LE. clear H.
+          apply Nat.sub_0_le, full_states_no_ce in LE; auto.
+          now rewrite Heq in LE.
+        + assert (Hce : output_string (make_moore t) s <> output_lang s)
+            by now apply equiv_query_ce.
+          pose proof Hwf as Hwf'.
+          destruct Hwf' as (Hwf' & Heps).
+          destruct (find_split t s Heps
+                      (wf_consistent t Hwf)
+                      (wf_NoDup t Hwf)
+                      Hce)
+              as (target & e & q_new &
+                  HinT & Hfresh & Hdiff &
+                  Hwf'' & Heps').
+          enough (L.num_states_in_minimal -
+                  List.length (leaves (ttt_step t target e q_new)) <= n).
+          eapply (ttt_learn n (ttt_step t target e q_new) H),
+            finalize_preserves_wf. now split.
+          unfold ttt_step.
+          pose proof
+            (split_leaf_count t target e q_new
+                (wf_NoDup t Hwf) HinT Hfresh) as Hcount.
+          rewrite finalize_leaves, Hcount. lia.
+    - eexists. exists (make_moore t). now apply make_moore_minimal.
+  Defined.
+
+  Definition mttt (_ : unit) : { St : Type & {m : M.t St | minimal m} } :=
+    ttt_learn num_states_in_minimal (Leaf nil) ltac:(lia) (conj I (or_introl eq_refl)).
+
+End Learner.
+
+End TTT_Moore_Binary.
